Add `fresh_loc`

ulib/LowStar.Monotonic.Buffer.fsti
@@ -1575,6 +1575,20 @@ val modifies_inert_loc_unused_in
     [SMTPat (modifies_inert l h1 h2); SMTPat (loc_unused_in h1 `loc_includes` l')];
   ]]
 
+/// Shorthand: freshness
+
+let fresh_loc (l: loc) (h h' : HS.mem) : GTot Type0 =
+  loc_unused_in h `loc_includes` l /\
+  loc_not_unused_in h' `loc_includes` l
+
+let ralloc_post_fresh_loc (#a:Type) (#rel:Preorder.preorder a) (i: HS.rid) (init:a) (m0: HS.mem)
+                       (x: HST.mreference a rel{HS.is_eternal_region (HS.frameOf x)}) (m1: HS.mem) : Lemma
+    (requires (HST.ralloc_post i init m0 x m1))
+    (ensures (fresh_loc (loc_freed_mreference x) m0 m1))
+    [SMTPat (HST.ralloc_post i init m0 x m1)]
+=  ()
+
+
 /// Legacy shorthands for disjointness and inclusion of buffers
 ///
 
